Relocate prepare_procedures_memory_after_linking
Since our experimental definition appears by all measures to be going in
the right direction, replace the legacy definitions with the new ones
via renaming and integrate them, without changes, in the existing
proofs.

Intermediate/Machine.v
@@ -627,13 +627,13 @@ Proof.
   apply alloc_static_buffers_after_linking; auto.
 Qed.
 
+(*
 Definition prepare_procedures_memory (p: program) (mem: Memory.t) : Memory.t :=
   let '(mem, _, _) := prepare_procedures p mem in
   mem.
+*)
 
-(* Lemma placeholder: prepare_procedures_memory_after_linking *)
-
-Definition prepare_procedures_memory' (p: program) : Memory.t :=
+Definition prepare_procedures_memory (p: program) : Memory.t :=
   let '(mem, _, _) := prepare_procedures_initial_memory p in
   mem.
 
@@ -649,11 +649,11 @@ Proof.
 Admitted. (* Grade 1. *)
 
 (* Now it's easy to extend this to the parts of the final result. *)
-Lemma domm_prepare_procedures_memory': forall p,
-  domm (prepare_procedures_memory' p) = domm (prog_interface p).
+Lemma domm_prepare_procedures_memory: forall p,
+  domm (prepare_procedures_memory p) = domm (prog_interface p).
 Proof.
   intros p.
-  unfold prepare_procedures_memory', prepare_procedures_initial_memory.
+  unfold prepare_procedures_memory, prepare_procedures_initial_memory.
   rewrite domm_map.
   rewrite domm_prepare_procedures_initial_memory_aux.
   reflexivity.
@@ -685,17 +685,17 @@ Proof.
 Qed.
 
 (* RB: TODO: Simplify hypotheses if possible. *)
-Theorem prepare_procedures_memory_after_linking':
+Theorem prepare_procedures_memory_after_linking:
   forall p c,
     well_formed_program p ->
     well_formed_program c ->
     linkable (prog_interface p) (prog_interface c) ->
     linkable_mains p c ->
-    prepare_procedures_memory' (program_link p c) =
-    unionm (prepare_procedures_memory' p) (prepare_procedures_memory' c).
+    prepare_procedures_memory (program_link p c) =
+    unionm (prepare_procedures_memory p) (prepare_procedures_memory c).
 Proof.
   intros p c Hwfp Hwfc Hlinkable Hmains.
-  unfold prepare_procedures_memory',
+  unfold prepare_procedures_memory,
          prepare_procedures_initial_memory, prepare_procedures_initial_memory_aux.
   (* Peel off the top-level maps. *)
   rewrite <- mapm_unionm.
@@ -772,7 +772,7 @@ Proof.
       * reflexivity.
     + simpl. rewrite Hmainp Hmainc. reflexivity.
     + simpl. rewrite Hmainp Hmainc. reflexivity. (* Easy case. *)
-Admitted.
+Admitted. (* Grade 2. A few easy admits and "the issue". *)
 
 Definition prepare_procedures_entrypoints (p: program) (mem: Memory.t) : EntryPoint.t :=
   let '(_, _, entrypoints) := prepare_procedures p mem in
